
\documentclass [10pt,a4paper]{book}

\usepackage{amsmath}
\usepackage{amssymb}
\usepackage{graphicx}
\begin{document}
	
\begin{flushright}
Contert-fice Grannar \textbf{$\mid 327$}
\end{flushright}
\textbf{Solution:} All the prochctions in the grammar are not in CNF. We have to convert them into CNF keeping the language 
generating power the same.
Let us replace 'a' by $\mathrm{D}_{a}, \mathrm{~b}$ ' by $\mathrm{D}_{b}$, and ' $\mathrm{c}$ ' by $\mathrm{D}_{c}$. So, three new productions $\mathrm{D}_{\mathrm{a}} \rightarrow \mathrm{a}, \mathrm{D}_{\mathrm{b}} \rightarrow \mathrm{b},$ and$\mathrm{D}_{c} \rightarrow \mathrm{c}$ are added to the grammar. By replacing 'a' by $\mathrm{D}_{a}$, ' $\mathrm{'b'}$ by $\mathrm{D}_{b}$, and ' $\mathrm{'c'}$ by $\mathrm{D}_{c}$, and adding three productions, the modified grammar becomes
$$
\begin{array}{l}
	\mathrm{S} \rightarrow \mathrm{ABD_{a}} \\
	\mathrm{A} \rightarrow \mathrm{DaD_{a}} \mathrm{D_{b}} \\
	\mathrm{B} \rightarrow \mathrm{AD_{c}} \\
	\mathrm{D}_{a} \rightarrow \mathrm{a} \\
	\mathrm{D}_{b} \rightarrow \mathrm{b} \\
	\mathrm{D}_{c} \rightarrow \mathrm{c}
\end{array}
$$
$\mathrm{S} \rightarrow \mathrm{ABDa}$ and $\mathrm{A} \rightarrow \mathrm{Da} \mathrm{DaDb}$ are not in CNF. Take two non-terminals $\mathrm{E}$ and $\mathrm{F}$. Replace $\mathrm{AB}$ by $\mathrm{E}$
and DaDa by F. So, two new productions $\mathrm{E} \rightarrow \mathrm{AB}$ and $\mathrm{F} \rightarrow$ DaDa will be added to the grammer.By replacement and adding the productions, the modified prammar will be

\begin{center}
	
$\mathrm{S} \rightarrow \mathrm{ABD_{a}}$

$\mathrm{A} \rightarrow \mathrm{DaD}_{a} \mathrm{D}_{b}$

$\mathrm{B} \rightarrow \mathrm{AD}_{\mathrm{c}}$

$\mathrm{D}_{a} \rightarrow \mathrm{a}$

$\mathrm{D}_{\mathrm{b}} \rightarrow \mathrm{b}$

$\mathrm{D}_{\mathrm{c}} \rightarrow \mathrm{c}$

$\mathrm{E} \rightarrow \mathrm{AB}$

$\mathrm{F} \rightarrow \mathrm{D}_{a} \mathrm{D}_{\mathrm{a}}$

\end{center}
In the previous grammar, all the productions are in the form of Non-terminal $\rightarrow$ string of exactly two non-terminals or non-terminal $\rightarrow$ single terminal. So, the grammar is in CNF.

\begin{flushleft}
\includegraphics[scale=0.5]{6.39}   Convert the following grammar into CNF.
\end{flushleft}
$$
\begin{array}{l}
	\mathrm{E} \rightarrow \mathrm{E}+\mathrm{E} \\
	\mathrm{E} \rightarrow \mathrm{E} ^* \mathrm{E} \\
	\mathrm{E} \rightarrow \mathrm{id}
\end{array}
$$
where $\Sigma=(+, ^*,$ id $)$ 

\begin{flushleft}
	
\textbf{Solution:} Except $\mathrm{E} \rightarrow$ id, all the other productions of the grammar are not in CNF. In the grammar $\mathrm{E} \rightarrow \mathrm{E}+\mathrm{E}$ and $\mathrm{E} \rightarrow \mathrm{E}  ^*\mathrm{E}$, there are two terminals $+$ and $^*$. Take two non-terminals $\mathrm{C}$ and $\mathrm{D}$ for replacing + and $^*$, respectively. Two new productions will be added to the grammar. By replacing + and $*$, the modified production rules will be
$$
\begin{array}{l}
	E \rightarrow E C E \\
	E \rightarrow E D E \\
	E \rightarrow i d \\
	C \rightarrow+ \\
	D \rightarrow^*
\end{array}
$$
In the production rules $E \rightarrow E C E$ and $E \rightarrow E D E$, there are three non-terminals. Replace $E C$ by another non-terminal $F$ and ED by G. So, two new productions $F \rightarrow E C$ and $G \rightarrow E D$ will be added to the grammar. By replacing and adding the new productions, the modified prammar will be

\end{flushleft}
\end{document}