
\documentclass [10pt,a4paper]{book}

\usepackage{amsmath}
\usepackage{amssymb}
\usepackage{graphicx}
\begin{document}
	
\begin{flushleft}
	
\textbf{$ 328 \mid$} Intreduction to hutomata Theory, formal Languages and Conputation
\end{flushleft}
$$
\begin{array}{l}
	E \rightarrow F E \\
	E \rightarrow G E \\
	E \rightarrow i d \\
	C \rightarrow+ \\
	D \rightarrow * \\
	F \rightarrow E C \\
	G \rightarrow E D
\end{array}
$$
In the previous grammar, all the productions are in the form of non-terminal $\rightarrow$ string of exactly two non-terminals or non-terminal $\rightarrow$ single terminal. So, the mammar is in CNF.


\begin{flushleft}
\includegraphics[scale=0.5]{6.40} Comvert the following grammar into CNF.
\end{flushleft}
$$
\begin{array}{l}
	S \rightarrow \operatorname{abAB} \\
	A \rightarrow \operatorname{bAB} / \in \\
	B \rightarrow b A a /\in
\end{array}
$$
\textbf{Solution:} In the mammar, there are two mil prodnctions $A \rightarrow \in$ and $B \rightarrow \in$ First, these productions must be removed, and after that the grammar can be converted into CNF. After removing the mill production $A \rightarrow \in$, the modified grammar becomes


$$
\begin{array}{l}
	\mathrm{S} \rightarrow \mathrm{abAB} / \mathrm{abB} \\
	\mathrm{A} \rightarrow \mathrm{bAB} / \mathrm{bB} \\
	\mathrm{B} \rightarrow \mathrm{Ba}
\end{array}
$$

After removine the null production $\mathrm{B} \rightarrow \in$, the modified mammar becomes
$$
\begin{array}{l}
	S \rightarrow \operatorname{abAB} / a b A / a b B / a b \\
	A \rightarrow b A B / b A / b B / b \\
	B \rightarrow B a / A a / a
\end{array}
$$
Now, this grammar can be converted into CNF. In the grammar, except $A \rightarrow b$ and $B \rightarrow a$, all the productions are not in CNF. Let us take two non-terminals $\mathrm{C}_{\mathrm{a}}$ and $\mathrm{C}_{\mathrm{b}}$ which will replace a and $\mathrm{b}$, respectively. So, two new productions $\mathrm{C}_{\mathrm{a}} \rightarrow \mathrm{a}$ and $\mathrm{C}_{\mathrm{b}} \rightarrow \mathrm{b}$ will be added to the grammar. After replacing and adding new productions, the modified grammar is
$$
\begin{array}{l}
	\mathrm{S} \rightarrow \mathrm{CaC_{b}} \mathrm{AB} / \mathrm{C}_{a} \mathrm{C}_{\mathrm{b}} \mathrm{A} / \mathrm{C}_{\mathrm{a}} \mathrm{C}_{\mathrm{b}} \mathrm{B} / \mathrm{C}_{a} \mathrm{C}_{b} \\
	\mathrm{~A} \rightarrow \mathrm{C}_{\mathrm{b}} \mathrm{AB} / \mathrm{C}_{\mathrm{b}} \mathrm{A} / \mathrm{C}_{\mathrm{b}} \mathrm{B} / \mathrm{b} \\
	\mathrm{B} \rightarrow \mathrm{BC_{a}} / \mathrm{ACa} / \mathrm{a} \\
	\mathrm{C}_{a} \rightarrow \mathrm{a} \\
	\mathrm{C}_{\mathrm{b}} \rightarrow \mathrm{b}
\end{array}
$$





In this modified grammar, $\mathrm{S} \rightarrow \mathrm{CaC}_{\mathrm{b}} \mathrm{AB}, \mathrm{S} \rightarrow \mathrm{Ca} \mathrm{CbA}, \mathrm{S} \rightarrow \mathrm{Ca} \mathrm{C}_{\mathrm{b}} \mathrm{B},$ and $\mathrm{A} \rightarrow \mathrm{C}_{\mathrm{b}} \mathrm{AB}$ are not in
CNF. Let us take two other non-terminals $D$ and $E$, which will be replaced in the place of $C a C_{b}$ and $A B$, respectively. So, two new productions $\mathrm{D} \rightarrow \mathrm{CaC}_{\mathrm{b}}$ and $\mathrm{E} \rightarrow \mathrm{AB}$ will be added to the grammar. By replacing and adding two new productions, the modified grammar is
$$
\begin{array}{l}
	\mathrm{S} \rightarrow \mathrm{DE} / \mathrm{DA} / \mathrm{DB} / \mathrm{C}_{\mathrm{a}} \mathrm{C}_{\mathrm{b}} \\
	\mathrm{A} \rightarrow \mathrm{C}_{\mathrm{b}} \mathrm{E}/ \mathrm{C}_{\mathrm{b}} \mathrm{A} / \mathrm{C}_{\mathrm{b}} \mathrm{B} / \mathrm{b} \\
	\mathrm{B} \rightarrow \mathrm{BCa} / \mathrm{ACa} / \mathrm{a}
\end{array}
$$






















\end{document}